Stick an uncurry pass in the pipeline
This allows us to (a) consolidate the constant and non-constant
pipelines and (b) vastly simplify the call-with-id-continuation logic.

src/Experiments/SimplyTypedArithmetic.v
@@ -501,11 +501,10 @@ Section mod_ops.
   Qed.
 
   Derive carry_mulmod
-         SuchThat (forall (fg : list Z * list Z)
-                          (f := fst fg) (g := snd fg)
+         SuchThat (forall (f g : list Z)
                           (Hf : length f = n)
                           (Hg : length g = n),
-                      (eval weight n (carry_mulmod fg)) mod (s - Associational.eval c)
+                      (eval weight n (carry_mulmod f g)) mod (s - Associational.eval c)
                       = (eval weight n f * eval weight n g) mod (s - Associational.eval c))
          As eval_carry_mulmod.
   Proof.
@@ -516,7 +515,7 @@ Section mod_ops.
           by auto; reflexivity ].
     eapply f_equal2; [|trivial]. eapply f_equal.
     expand_lists ().
-    subst f g carry_mulmod; reflexivity.
+    subst carry_mulmod; reflexivity.
   Qed.
 
   Derive carrymod
@@ -536,11 +535,10 @@ Section mod_ops.
   Qed.
 
   Derive addmod
-         SuchThat (forall (fg: list Z * list Z)
-                          (f := fst fg) (g := snd fg)
+         SuchThat (forall (f g : list Z)
                           (Hf : length f = n)
                           (Hg : length g = n),
-                      (eval weight n (addmod fg)) mod (s - Associational.eval c)
+                      (eval weight n (addmod f g)) mod (s - Associational.eval c)
                       = (eval weight n f + eval weight n g) mod (s - Associational.eval c))
          As eval_addmod.
   Proof.
@@ -548,16 +546,15 @@ Section mod_ops.
     rewrite <-eval_add by auto.
     eapply f_equal2; [|trivial]. eapply f_equal.
     expand_lists ().
-    subst f g addmod; reflexivity.
+    subst addmod; reflexivity.
   Qed.
 
   Derive submod
          SuchThat (forall (coef:Z)
-                          (fg: list Z * list Z)
-                          (f := fst fg) (g := snd fg)
+                          (f g : list Z)
                           (Hf : length f = n)
                           (Hg : length g = n),
-                      (eval weight n (submod coef fg)) mod (s - Associational.eval c)
+                      (eval weight n (submod coef f g)) mod (s - Associational.eval c)
                       = (eval weight n f - eval weight n g) mod (s - Associational.eval c))
          As eval_submod.
   Proof.
@@ -565,7 +562,7 @@ Section mod_ops.
     rewrite <-eval_sub with (coef:=coef) by auto.
     eapply f_equal2; [|trivial]. eapply f_equal.
     expand_lists ().
-    subst f g submod; reflexivity.
+    subst submod; reflexivity.
   Qed.
 
   Derive oppmod
@@ -1634,17 +1631,17 @@ Module Ring.
                 is_bounded_by tight_bounds arg = true
                 -> is_bounded_by loose_bounds (Interp_rrelaxv arg) = true
                    /\ Interp_rrelaxv arg = expanding_id n arg)
-            (carry_mulmod : list Z * list Z -> list Z)
+            (carry_mulmod : list Z -> list Z -> list Z)
             (Hcarry_mulmod
-             : forall fg,
-                length (fst fg) = n -> length (snd fg) = n ->
-                (eval (carry_mulmod fg)) mod (s - Associational.eval c)
-                = (eval (fst fg) * eval (snd fg)) mod (s - Associational.eval c))
+             : forall f g,
+                length f = n -> length g = n ->
+                (eval (carry_mulmod f g)) mod (s - Associational.eval c)
+                = (eval f * eval g) mod (s - Associational.eval c))
             (Interp_rcarry_mulv : list Z * list Z -> list Z)
             (HInterp_rcarry_mulv : forall arg,
                 is_bounded_by2 loose_bounds arg = true
                 -> is_bounded_by tight_bounds (Interp_rcarry_mulv arg) = true
-                   /\ Interp_rcarry_mulv arg = carry_mulmod arg)
+                   /\ Interp_rcarry_mulv arg = carry_mulmod (fst arg) (snd arg))
             (carrymod : list Z -> list Z)
             (Hcarrymod
              : forall f,
@@ -1656,28 +1653,28 @@ Module Ring.
                 is_bounded_by loose_bounds arg = true
                 -> is_bounded_by tight_bounds (Interp_rcarryv arg) = true
                    /\ Interp_rcarryv arg = carrymod arg)
-            (addmod : list Z * list Z -> list Z)
+            (addmod : list Z -> list Z -> list Z)
             (Haddmod
-             : forall fg,
-                length (fst fg) = n -> length (snd fg) = n ->
-                (eval (addmod fg)) mod (s - Associational.eval c)
-                = (eval (fst fg) + eval (snd fg)) mod (s - Associational.eval c))
+             : forall f g,
+                length f = n -> length g = n ->
+                (eval (addmod f g)) mod (s - Associational.eval c)
+                = (eval f + eval g) mod (s - Associational.eval c))
             (Interp_raddv : list Z * list Z -> list Z)
             (HInterp_raddv : forall arg,
                 is_bounded_by2 tight_bounds arg = true
                 -> is_bounded_by loose_bounds (Interp_raddv arg) = true
-                   /\ Interp_raddv arg = addmod arg)
-            (submod : list Z * list Z -> list Z)
+                   /\ Interp_raddv arg = addmod (fst arg) (snd arg))
+            (submod : list Z -> list Z -> list Z)
             (Hsubmod
-             : forall fg,
-                length (fst fg) = n -> length (snd fg) = n ->
-                (eval (submod fg)) mod (s - Associational.eval c)
-                = (eval (fst fg) - eval (snd fg)) mod (s - Associational.eval c))
+             : forall f g,
+                length f = n -> length g = n ->
+                (eval (submod f g)) mod (s - Associational.eval c)
+                = (eval f - eval g) mod (s - Associational.eval c))
             (Interp_rsubv : list Z * list Z -> list Z)
             (HInterp_rsubv : forall arg,
                 is_bounded_by2 tight_bounds arg = true
                 -> is_bounded_by loose_bounds (Interp_rsubv arg) = true
-                   /\ Interp_rsubv arg = submod arg)
+                   /\ Interp_rsubv arg = submod (fst arg) (snd arg))
             (oppmod : list Z -> list Z)
             (Hoppmod
              : forall f,
@@ -1773,10 +1770,12 @@ Module Ring.
                | [ |- _ = _ :> Z ] => first [ reflexivity | rewrite <- m_eq; reflexivity ]
                | [ H : context[?x] |- Fdecode ?x = _ ] => rewrite H
                | [ H : context[?x _] |- Fdecode (?x _) = _ ] => rewrite H
+               | [ H : context[?x _ _] |- Fdecode (?x _ _) = _ ] => rewrite H
                | _ => progress cbv [Fdecode]
                | [ |- _ = _ :> F _ ] => apply F.eq_to_Z_iff
                | _ => progress autorewrite with push_FtoZ
                | _ => rewrite m_eq
+               | [ H : context[?x _ _] |- context[eval (?x _ _)] ] => rewrite H
                | [ H : context[?x _] |- context[eval (?x _)] ] => rewrite H
                | [ H : context[?x] |- context[eval ?x] ] => rewrite H
                | [ |- context[List.length ?x] ]
@@ -4187,347 +4186,69 @@ Module Compilers.
         : @Compilers.Uncurried.expr.default.Expr R
         := expr.CallWithContinuation (@ident.untranslate _) (@ident.fst) (@ident.snd) e k.
 
-      (** It's not clear how to "plug in the identity continuation"
-          for the CPS'd form of an expression of type [((A -> B) -> C)
-          -> D].  So we must describe types of at most second order
-          functions, so that we can write a uniform "plug in the
-          identity continuation" transformation. *)
-      Module second_order.
-        Import Compilers.type.
-        Module Import type.
-          Inductive flat_type :=
-          | type_primitive (_ : primitive)
-          | prod (_ : flat_type) (_ : flat_type)
-          | list (_ : flat_type).
-          Inductive argtype :=
-          | flat_arg (_ : flat_type)
-          | arrow_arg (s : flat_type) (d : argtype)
-          | prod_arg (_ _ : argtype).
-          Inductive type :=
-          | flat (_ : flat_type)
-          | arrow (s : argtype) (d : type).
-        End type.
-
-        Module Export Coercions.
-          Coercion type_primitive : primitive >-> flat_type.
-          Coercion flat_arg : flat_type >-> argtype.
-          Coercion flat : flat_type >-> type.
-        End Coercions.
-        Notation flat_type := flat_type.
-        Notation argtype := argtype.
-        Notation type := type.
-
-        Fixpoint flat_to_type (t : flat_type) : Compilers.type.type
-          := match t with
-             | type_primitive x => x
-             | prod A B => Compilers.type.prod (flat_to_type A) (flat_to_type B)
-             | list A => Compilers.type.list (flat_to_type A)
-             end.
-
-        Fixpoint arg_to_type (t : argtype) : Compilers.type.type
-          := match t with
-             | flat_arg t => flat_to_type t
-             | arrow_arg s d => Compilers.type.arrow (flat_to_type s) (arg_to_type d)
-             | prod_arg A B => Compilers.type.prod (arg_to_type A) (arg_to_type B)
-             end.
-
-        Fixpoint to_type (t : type) : Compilers.type.type
-          := match t with
-             | flat t => flat_to_type t
-             | arrow s d => Compilers.type.arrow (arg_to_type s) (to_type d)
-             end.
-
-        Fixpoint flat_of_type (t : Compilers.type.type) : option flat_type
-          := match t with
-             | Compilers.type.type_primitive x => @Some flat_type x
-             | Compilers.type.prod A B
-               => match flat_of_type A, flat_of_type B with
-                  | Some A, Some B => @Some flat_type (prod A B)
-                  | _, _ => None
-                  end
-             | Compilers.type.arrow s d => None
-             | Compilers.type.list A
-               => option_map list (flat_of_type A)
-             end.
-
-        Fixpoint arg_of_type (t : Compilers.type.type) : option argtype
-          := match t with
-             | Compilers.type.prod A B as t
-               => match flat_of_type t, arg_of_type A, arg_of_type B with
-                  | Some t, _, _
-                    => @Some argtype t
-                  | None, Some A, Some B
-                    => @Some argtype (prod_arg A B)
-                  | _, _, _ => None
-                  end
-             | Compilers.type.arrow s d
-               => match flat_of_type s, arg_of_type d with
-                  | Some s, Some d => Some (arrow_arg s d)
-                  | _, _ => None
-                  end
-             | Compilers.type.type_primitive _ as t
-             | Compilers.type.list _ as t
-               => option_map flat_arg (flat_of_type t)
-             end.
-
-        Fixpoint of_type (t : Compilers.type.type) : option type
-          := match t with
-             | Compilers.type.arrow s d
-               => match arg_of_type s, of_type d with
-                  | Some s, Some d => Some (arrow s d)
-                  | _, _ => None
-                  end
-             | Compilers.type.prod _ _ as t
-             | Compilers.type.type_primitive _ as t
-             | Compilers.type.list _ as t
-               => option_map flat (flat_of_type t)
-             end.
-
-        Fixpoint try_transport_flat_of_type P (t : Compilers.type.type)
-          : P t -> option { t' : _ & P (flat_to_type t') }
-          := match t with
-             | Compilers.type.type_primitive x
-               => fun v => Some (existT _ (x : flat_type) v)
-             | Compilers.type.prod A B
-               => fun v
-                  => match try_transport_flat_of_type (fun a => P (a * _)%ctype) A v with
-                     | Some (existT A v)
-                       => match try_transport_flat_of_type (fun b => P (_ * b)%ctype) B v with
-                          | Some (existT B v)
-                            => Some (existT _ (prod A B) v)
-                          | None => None
-                          end
-                     | None => None
-                     end
-             | Compilers.type.arrow s d => fun _ => None
-             | Compilers.type.list A
-               => fun v
-                  => option_map
-                       (fun '(existT A v) => existT (fun t => P (flat_to_type t)) (list A) v)
-                       (try_transport_flat_of_type (fun a => P (Compilers.type.list a)) A v)
-             end.
-
-        Fixpoint try_transport_arg_of_type P (t : Compilers.type.type)
-          : P t -> option { t' : _ & P (arg_to_type t') }
-          := match t with
-             | Compilers.type.prod A B as t
-               => fun v
-                  => match try_transport_flat_of_type P t v with
-                     | Some (existT t v) => Some (existT (fun t' => P (arg_to_type t')) t v)
-                     | None
-                       => match try_transport_arg_of_type (fun a => P (a * _)%ctype) A v with
-                          | Some (existT A v)
-                            => match try_transport_arg_of_type (fun b => P (_ * b)%ctype) B v with
-                               | Some (existT B v)
-                                 => Some (existT _ (prod_arg A B) v)
-                               | None => None
-                               end
-                          | None => None
-                          end
-                     end
-             | Compilers.type.arrow s d
-               => fun v
-                  => match try_transport_flat_of_type (fun s => P (s -> _)%ctype) s v with
-                     | Some (existT s v)
-                       => match try_transport_flat_of_type (fun d => P (_ -> d)%ctype) d v with
-                          | Some (existT d v)
-                            => Some (existT (fun t' => P (arg_to_type t')) (arrow_arg s d) v)
-                          | None => None
-                          end
-                     | None => None
-                     end
-             | Compilers.type.type_primitive _ as t
-             | Compilers.type.list _ as t
-               => fun v
-                  => option_map
-                       (fun '(existT t v) => existT (fun t => P (arg_to_type t)) (flat_arg t) v)
-                       (try_transport_flat_of_type P t v)
-             end.
-
-        Fixpoint try_transport_of_type P (t : Compilers.type.type)
-          : P t -> option { t' : _ & P (to_type t') }
-          := match t with
-             | Compilers.type.arrow s d
-               => fun v
-                  => match try_transport_arg_of_type (fun s => P (s -> _)%ctype) s v with
-                     | Some (existT s v)
-                       => match try_transport_of_type (fun d => P (_ -> d)%ctype) d v with
-                          | Some (existT d v)
-                            => Some (existT (fun t' => P (to_type t')) (arrow s d) v)
-                          | None => None
-                          end
-                     | None => None
-                     end
-             | Compilers.type.prod _ _ as t
-             | Compilers.type.type_primitive _ as t
-             | Compilers.type.list _ as t
-               => fun v
-                  => option_map
-                       (fun '(existT t v) => existT (fun t => P (to_type t)) (flat t) v)
-                       (try_transport_flat_of_type P t v)
-             end.
-      End second_order.
-      Import second_order.Coercions.
-
-      Fixpoint untranslate_translate_flat
-               (P : Compilers.type.type -> Type)
-               {R}
-               {t : second_order.flat_type}
-               (e : P (second_order.to_type t))
-               {struct t}
-        : P (type.untranslate R (type.translate (second_order.to_type t)))
-        := match t return P (second_order.to_type t)
-                          -> P (type.untranslate R (type.translate (second_order.to_type t)))
-           with
-           | second_order.type.type_primitive x => id
-           | second_order.type.prod A B
-             => fun ab : P (second_order.flat_to_type A * second_order.flat_to_type B)%ctype
-                => @untranslate_translate_flat
-                     (fun a => P (a * _)%ctype)
-                     R A
-                     (@untranslate_translate_flat
-                        (fun b => P (_ * b)%ctype)
-                        R B
-                        ab)
-           | second_order.type.list A
-             => @untranslate_translate_flat
-                  (fun t => P (Compilers.type.list t))
-                  R A
-           end e.
-
-      Fixpoint untranslate_translate_flat'
-               (P : Compilers.type.type -> Type)
-               {R}
-               {t : second_order.flat_type}
-               (e : P (type.untranslate R (type.translate (second_order.to_type t))))
-               {struct t}
-        : P (second_order.to_type t)
-        := match t return P (type.untranslate R (type.translate (second_order.to_type t)))
-                          -> P (second_order.to_type t)
-           with
-           | second_order.type.type_primitive x => id
-           | second_order.type.prod A B
-             => fun ab :
-                      (* ignore this line *) P (type.untranslate R (type.translate (second_order.flat_to_type A)) * type.untranslate R (type.translate (second_order.flat_to_type B)))%ctype
-                => @untranslate_translate_flat'
-                     (fun a => P (a * _)%ctype)
-                     R A
-                     (@untranslate_translate_flat'
-                        (fun b => P (_ * b)%ctype)
-                        R B
-                        ab)
-           | second_order.type.list A
-             => @untranslate_translate_flat'
-                  (fun t => P (Compilers.type.list t))
-                  R A
-           end e.
-
-      Definition transport_final_codomain_flat P {t}
-        : P (second_order.flat_to_type t)
-          -> P (type.final_codomain (second_order.flat_to_type t))
-        := match t with
-           | second_order.type.type_primitive x => id
-           | second_order.type.prod x x0 => id
-           | second_order.type.list x => id
+      Local Notation iffT A B := ((A -> B) * (B -> A))%type.
+      (** We can only "plug in the identity continuation" for flat
+          (arrow-free) types.  (Actually, we know how to do it in a
+          very ad-hoc way for types of at-most second-order functions;
+          see git history.  This is much simpler.) *)
+      Fixpoint try_untranslate_translate {R} {t}
+        : option (forall (P : Compilers.type.type -> Type),
+                     iffT (P (type.untranslate R (type.translate t))) (P t))
+        := match t return option (forall (P : Compilers.type.type -> Type),
+                                     iffT (P (type.untranslate R (type.translate t))) (P t)) with
+           | Compilers.type.type_primitive x
+             => Some (fun P => ((fun v => v), (fun v => v)))
+           | type.arrow s d => None
+           | Compilers.type.prod A B
+             => (fA <- (@try_untranslate_translate _ A);
+                   fB <- (@try_untranslate_translate _ B);
+                   Some
+                     (fun P
+                      => let fA := fA (fun A => P (Compilers.type.prod A (type.untranslate R (type.translate B)))) in
+                         let fB := fB (fun B => P (Compilers.type.prod A B)) in
+                         ((fun v => fst fB (fst fA v)),
+                          (fun v => snd fA (snd fB v)))))%option
+           | Compilers.type.list A
+             => (fA <- (@try_untranslate_translate R A);
+                   Some (fun P => fA (fun A => P (Compilers.type.list A))))%option
            end.
-
-      Definition transport_final_codomain_flat' P {t}
-        : P (type.final_codomain (second_order.flat_to_type t))
-          -> P (second_order.flat_to_type t)
-        := match t with
-           | second_order.type.type_primitive x => id
-           | second_order.type.prod x x0 => id
-           | second_order.type.list x => id
-           end.
-
-      Fixpoint untranslate_translate_arg
-               {var}
-               {R}
-               {t : second_order.argtype}
-               (e : @Compilers.Uncurried.expr.default.expr var (second_order.arg_to_type t))
-               {struct t}
-        : @Compilers.Uncurried.expr.default.expr var (type.untranslate R (type.translate (second_order.arg_to_type t)))
-        := match t return Compilers.Uncurried.expr.default.expr (second_order.arg_to_type t)
-                          -> Compilers.Uncurried.expr.default.expr (type.untranslate R (type.translate (second_order.arg_to_type t)))
-           with
-           | second_order.type.flat_arg t
-             => untranslate_translate_flat _
-           | second_order.type.arrow_arg s d
-             => fun e'
-                => Abs (fun v :
-                              (* ignore this line *) var (type.untranslate R (type.translate (second_order.flat_to_type s)) * (type.untranslate R (type.translate (second_order.arg_to_type d)) -> R))%ctype
-                        => (ident.snd @@ Var v)
-                             @ (@untranslate_translate_arg
-                                  var R d
-                                  (e' @ (untranslate_translate_flat' _ (ident.fst @@ Var v)))))%expr
-           | second_order.type.prod_arg A B
-             => fun e' : expr.default.expr (second_order.arg_to_type A * second_order.arg_to_type B)
-                => ((Abs (fun a => Abs (fun b => (Var a, Var b))))
-                      @ (@untranslate_translate_arg var R A (ident.fst @@ e'))
-                      @ (@untranslate_translate_arg var R B (ident.snd @@ e')))%expr
-           end e.
 
       Local Notation "x <-- e1 ; e2" := (expr.splice e1 (fun x => e2%cpsexpr)) : cpsexpr_scope.
 
-      Fixpoint call_fun_with_id_continuation'
-               {var}
-               {t : second_order.type}
-               (R := type.final_codomain (second_order.to_type t))
-               (e : @expr (fun t0 =>
-                             @Uncurried.expr.expr default.ident.ident var (type.untranslate R t0))
-                          (type.translate (second_order.to_type t)))
-               {struct t}
-        : @Compilers.Uncurried.expr.default.expr var (second_order.to_type t)
-        := match t
-                 return (@expr (fun t0 =>
-                                  @Uncurried.expr.expr default.ident.ident var (type.untranslate (type.final_codomain (second_order.to_type t)) t0))
-                               (type.translate (second_order.to_type t)))
-                        -> @Compilers.Uncurried.expr.default.expr var (second_order.to_type t)
-           with
-           | second_order.type.flat t
-             => fun e'
-                => transport_final_codomain_flat'
-                     _
-                     (@call_with_continuation
-                        var _ _ e'
-                        (fun e'' => transport_final_codomain_flat _ (untranslate_translate_flat' _ e'')))
-           | second_order.type.arrow s d
-             => fun e' :
-                      (* ignore this line *) expr (type.translate (second_order.arg_to_type s) * (type.translate (second_order.to_type d) --->) --->)
-                => Abs (s:=second_order.arg_to_type s) (d:=second_order.to_type d)
-                       (fun v
-                        => @call_fun_with_id_continuation'
-                             var d
-                             (f <-- e';
+      Definition call_fun_with_id_continuation'
+                 {s d}
+        : option (forall var
+                         (e : @expr _ (type.translate (s -> d))),
+                     @Compilers.Uncurried.expr.default.expr var (s -> d))
+        := (fs <- (@try_untranslate_translate _ s);
+              fd <- (@try_untranslate_translate _ d);
+              Some
+                (fun var e
+                 => let P := @Compilers.Uncurried.expr.default.expr var in
+                    Abs
+                      (fun v : var s
+                       => call_with_continuation
+                            ((f <-- e;
                                 k <- (λ r, expr.Halt r);
-                                p <- (untranslate_translate_arg (Var v), k);
+                                p <- (snd (fs P) (Var v), k);
                                 f @ p)%cpsexpr)
-           end e.
-      Definition CallFunWithIdContinuation'
-                 {t : second_order.type}
-                 (e : Expr (type.translate (second_order.to_type t)))
-        : @Compilers.Uncurried.expr.default.Expr (second_order.to_type t)
-        := fun var => @call_fun_with_id_continuation' _ t (e _).
+                            (fst (fd P)))))%option.
+
+      Definition call_fun_with_id_continuation
+                 {var}
+                 {s d} (e : @expr _ (type.translate (s -> d)))
+        : option (@Compilers.Uncurried.expr.default.expr var (s -> d))
+        := option_map
+             (fun f => f _ e)
+             (@call_fun_with_id_continuation' s d).
 
       Definition CallFunWithIdContinuation
-                 {t}
-                 (e : Expr (type.translate t))
-        := match second_order.try_transport_of_type (fun t => Expr (type.translate t)) _
-                                                  e
-                 as o return match o with None => _ | _ => _ end
-           with
-           | Some v => CallFunWithIdContinuation' (projT2 v)
-           | None => I
-           end.
-
-      Definition CallFunWithIdContinuation_opt
-                 {t}
-                 (e : Expr (type.translate t))
-        : option (@Compilers.Uncurried.expr.default.Expr t)
-        := (e' <- (second_order.try_transport_of_type
-                     (fun t => Expr (type.translate t)) _
-                     e);
-              type.try_transport _ _ _ (CallFunWithIdContinuation' (projT2 e')))%option.
+                 {s d}
+                 (e : Expr (type.translate (s -> d)))
+        : option (@Compilers.Uncurried.expr.default.Expr (s -> d))
+        := option_map
+             (fun f var => f _ (e _))
+             (@call_fun_with_id_continuation' s d).
     End default.
     Include default.
   End CPS.
@@ -6404,19 +6125,20 @@ Module test3.
                         (z * z)) in
     pose v as E.
     vm_compute in E.
-    pose (PartialEvaluate false (CPS.CallFunWithIdContinuation (CPS.Translate (canonicalize_list_recursion E)))) as E'.
+    pose (option_map (PartialEvaluate false) (CPS.CallFunWithIdContinuation (CPS.Translate (canonicalize_list_recursion E)))) as E'.
     vm_compute in E'.
     lazymatch (eval cbv delta [E'] in E') with
-    | (fun var : type -> Type =>
-         (λ x : var (type.type_primitive type.Z),
-                expr_let x0 := Var x * Var x in
-              expr_let x1 := Var x0 * Var x0 in
-              expr_let x2 := Var x1 * Var x1 in
-              expr_let x3 := Var x2 * Var x2 in
-              Var x3 * Var x3)%expr)
+    | (Some
+         (fun var : type -> Type =>
+            (λ x : var (type.type_primitive type.Z),
+                   expr_let x0 := Var x * Var x in
+                 expr_let x1 := Var x0 * Var x0 in
+                 expr_let x2 := Var x1 * Var x1 in
+                 expr_let x3 := Var x2 * Var x2 in
+                 Var x3 * Var x3)%expr))
       => idtac
     end.
-    pose (PartialEvaluateWithBounds1 E' (Some r[0~>10]%zrange)) as E'''.
+    pose (PartialEvaluateWithBounds1 (invert_Some E') (Some r[0~>10]%zrange)) as E'''.
     lazy in E'''.
     lazymatch (eval cbv delta [E'''] in E''') with
     | (fun var : type -> Type =>
@@ -6441,10 +6163,10 @@ Module test4.
                         (xz :: xz :: nil)) in
     pose v as E.
     vm_compute in E.
-    pose (PartialEvaluate false (CPS.CallFunWithIdContinuation (CPS.Translate (canonicalize_list_recursion E)))) as E'.
+    pose (option_map (PartialEvaluate false) (CPS.CallFunWithIdContinuation (CPS.Translate (canonicalize_list_recursion E)))) as E'.
     lazy in E'.
     clear E.
-    pose (PartialEvaluateWithBounds1 E' (Some [Some r[0~>10]%zrange],Some [Some r[0~>10]%zrange])) as E''.
+    pose (PartialEvaluateWithBounds1 (invert_Some E') (Some [Some r[0~>10]%zrange],Some [Some r[0~>10]%zrange])) as E''.
     lazy in E''.
     lazymatch (eval cbv delta [E''] in E'') with
     | (fun var : type -> Type =>
@@ -6468,7 +6190,7 @@ Module test5.
                         x) in
     pose v as E.
     vm_compute in E.
-    pose (ReassociateSmallConstants.Reassociate (2^8) (PartialEvaluate false (CPS.CallFunWithIdContinuation (CPS.Translate (canonicalize_list_recursion E))))) as E'.
+    pose (ReassociateSmallConstants.Reassociate (2^8) (PartialEvaluate false (invert_Some (CPS.CallFunWithIdContinuation (CPS.Translate (canonicalize_list_recursion E)))))) as E'.
     lazy in E'.
     clear E.
     lazymatch (eval cbv delta [E'] in E') with
@@ -6495,7 +6217,7 @@ Module test6.
     pose (CPS.CallFunWithIdContinuation (CPS.Translate (canonicalize_list_recursion E))) as E'.
     lazy in E'.
     clear E.
-    pose (PartialEvaluate false E') as E''.
+    pose (PartialEvaluate false (invert_Some E')) as E''.
     lazy in E''.
     lazymatch eval cbv delta [E''] in E'' with
     | fun var : type -> Type => (λ x : var (type.type_primitive type.Z), Var x)%expr
@@ -6650,7 +6372,7 @@ Create HintDb reify_gen_cache.
 
 Derive carry_mul_gen
        SuchThat (forall (limbwidth_num limbwidth_den : Z)
-                        (fg : list Z * list Z)
+                        (f g : list Z)
                         (n : nat)
                         (s : Z)
                         (c : list (Z * Z))
@@ -6658,11 +6380,11 @@ Derive carry_mul_gen
                         (idxs : list nat)
                         (len_idxs : nat),
                     Interp (t:=type.reify_type_of carry_mulmod)
-                           carry_mul_gen limbwidth_num limbwidth_den s c n len_c idxs len_idxs fg
-                    = carry_mulmod limbwidth_num limbwidth_den s c n len_c idxs len_idxs fg)
+                           carry_mul_gen limbwidth_num limbwidth_den s c n len_c idxs len_idxs f g
+                    = carry_mulmod limbwidth_num limbwidth_den s c n len_c idxs len_idxs f g)
        As carry_mul_gen_correct.
 Proof. Time cache_reify (). exact admit. (* correctness of initial parts of the pipeline *) Time Qed.
-Hint Extern 1 (_ = carry_mulmod _ _ _ _ _ _ _ _ _) => simple apply carry_mul_gen_correct : reify_gen_cache.
+Hint Extern 1 (_ = carry_mulmod _ _ _ _ _ _ _ _ _ _) => simple apply carry_mul_gen_correct : reify_gen_cache.
 
 Derive carry_gen
        SuchThat (forall (limbwidth_num limbwidth_den : Z)
@@ -6696,14 +6418,14 @@ Hint Extern 1 (_ = encodemod _ _ _ _ _ _ _) => simple apply encode_gen_correct :
 
 Derive add_gen
        SuchThat (forall (limbwidth_num limbwidth_den : Z)
-                        (fg : list Z * list Z)
+                        (f g : list Z)
                         (n : nat),
                     Interp (t:=type.reify_type_of addmod)
-                           add_gen limbwidth_num limbwidth_den n fg
-                    = addmod limbwidth_num limbwidth_den n fg)
+                           add_gen limbwidth_num limbwidth_den n f g
+                    = addmod limbwidth_num limbwidth_den n f g)
        As add_gen_correct.
 Proof. cache_reify (). exact admit. (* correctness of initial parts of the pipeline *) Qed.
-Hint Extern 1 (_ = addmod _ _ _ _) => simple apply add_gen_correct : reify_gen_cache.
+Hint Extern 1 (_ = addmod _ _ _ _ _) => simple apply add_gen_correct : reify_gen_cache.
 Derive sub_gen
        SuchThat (forall (limbwidth_num limbwidth_den : Z)
                         (n : nat)
@@ -6711,13 +6433,13 @@ Derive sub_gen
                         (c : list (Z * Z))
                         (len_c : nat)
                         (coef : Z)
-                        (fg : list Z * list Z),
+                        (f g : list Z),
                     Interp (t:=type.reify_type_of submod)
-                           sub_gen limbwidth_num limbwidth_den s c n len_c coef fg
-                    = submod limbwidth_num limbwidth_den s c n len_c coef fg)
+                           sub_gen limbwidth_num limbwidth_den s c n len_c coef f g
+                    = submod limbwidth_num limbwidth_den s c n len_c coef f g)
        As sub_gen_correct.
 Proof. cache_reify (). exact admit. (* correctness of initial parts of the pipeline *) Qed.
-Hint Extern 1 (_ = submod _ _ _ _ _ _ _ _) => simple apply sub_gen_correct : reify_gen_cache.
+Hint Extern 1 (_ = submod _ _ _ _ _ _ _ _ _) => simple apply sub_gen_correct : reify_gen_cache.
 
 Derive opp_gen
        SuchThat (forall (limbwidth_num limbwidth_den : Z)
@@ -6773,6 +6495,7 @@ Derive id_gen
 Proof. cache_reify (). exact admit. (* correctness of initial parts of the pipeline *) Qed.
 Hint Extern 1 (_ = expanding_id _ _) => simple apply id_gen_correct : reify_gen_cache.
 
+Import Uncurry.
 Module Pipeline.
   Import GeneralizeVar.
   Inductive ErrorMessage :=
@@ -6808,16 +6531,17 @@ Module Pipeline.
       expr.Interp (@for_reification.ident.interp) E.
   Admitted.
 
-  Definition BoundsPipeline_0_or_1
+  Definition BoundsPipeline
              (with_dead_code_elimination : bool := true)
              (with_subst01 : bool)
+             relax_zrange
              {t}
              (E : Expr t)
-             {t'}
-             (CheckedPartialEvaluateWithBounds : _ -> _ -> _ + partial.data t')
+             arg_bounds
              out_bounds
-  : ErrorT (Expr t)
-    := let E := CPS.CallFunWithIdContinuation_opt (CPS.Translate E) in
+  : ErrorT (Expr (type.uncurry t))
+    := let E := expr.Uncurry E in
+       let E := CPS.CallFunWithIdContinuation (CPS.Translate E) in
        match E with
        | Some E
          => (let E := PartialEvaluate false E in
@@ -6832,7 +6556,7 @@ Module Pipeline.
              let E := FromFlat e in
              let E := if with_subst01 then Subst01.Subst01 E else E in
              let E := ReassociateSmallConstants.Reassociate (2^8) E in
-             let E := CheckedPartialEvaluateWithBounds E out_bounds in
+             let E := CheckedPartialEvaluateWithBounds1 relax_zrange E arg_bounds out_bounds in
              match E with
              | inl E => Success E
              | inr b
@@ -6841,45 +6565,14 @@ Module Pipeline.
        | None => Error (Type_too_complicated_for_cps t)
        end.
 
-  Definition BoundsPipeline
-             (with_dead_code_elimination : bool := true)
-             (with_subst01 : bool)
-             relax_zrange
-             {s d}
-             (E : Expr (s -> d))
-             arg_bounds
-             out_bounds
-    : ErrorT (Expr (s -> d))
-    := BoundsPipeline_0_or_1
-         (*with_dead_code_elimination*)
-         with_subst01
-         E
-         (fun E => CheckedPartialEvaluateWithBounds1 relax_zrange E arg_bounds)
-         out_bounds.
-
-  Definition BoundsPipelineConst
-             (with_dead_code_elimination : bool := true)
-             (with_subst01 : bool)
-             relax_zrange
-             {t}
-             (E : Expr t)
-             out_bounds
-    : ErrorT (Expr t)
-    := BoundsPipeline_0_or_1
-         (*with_dead_code_elimination*)
-         with_subst01
-         E
-         (fun E => CheckedPartialEvaluateWithBounds0 relax_zrange E)
-         out_bounds.
-
   Lemma BoundsPipeline_correct
              (with_dead_code_elimination : bool := true)
              (with_subst01 : bool)
              relax_zrange
              (Hrelax : forall r r' z : zrange,
                  (z <=? r)%zrange = true -> relax_zrange r = Some r' -> (z <=? r')%zrange = true)
-             {s d}
-             (e : Expr (s -> d))
+             {t}
+             (e : Expr t)
              arg_bounds
              out_bounds
              rv
@@ -6887,9 +6580,9 @@ Module Pipeline.
     : forall arg
              (Harg : ZRange.type.option.is_bounded_by arg_bounds arg = true),
       ZRange.type.option.is_bounded_by out_bounds (Interp rv arg) = true
-      /\ Interp rv arg = Interp e arg.
+      /\ Interp rv arg = app_curried (Interp e) arg.
   Proof.
-    cbv [BoundsPipeline BoundsPipeline_0_or_1 Let_In] in *;
+    cbv [BoundsPipeline Let_In] in *;
       repeat match goal with
              | [ H : match ?x with _ => _ end = Success _ |- _ ]
                => destruct x eqn:?; cbv beta iota in H; [ | congruence ];
@@ -6913,15 +6606,15 @@ Module Pipeline.
   Qed.
 
   Definition BoundsPipeline_correct_transT
-             {s d}
+             {t}
              arg_bounds
              out_bounds
-             (InterpE : type.interp s -> type.interp d)
-             (rv : Expr (s -> d))
+             (InterpE : type.interp t)
+             (rv : Expr (type.uncurry t))
     := forall arg
               (Harg : ZRange.type.option.is_bounded_by arg_bounds arg = true),
       ZRange.type.option.is_bounded_by out_bounds (Interp rv arg) = true
-      /\ Interp rv arg = InterpE arg.
+      /\ Interp rv arg = app_curried InterpE arg.
 
   Lemma BoundsPipeline_correct_trans
         (with_dead_code_elimination : bool := true)
@@ -6930,14 +6623,14 @@ Module Pipeline.
         (Hrelax
          : forall r r' z : zrange,
             (z <=? r)%zrange = true -> relax_zrange r = Some r' -> (z <=? r')%zrange = true)
-        {s d}
-        (e : Expr (s -> d))
+        {t}
+        (e : Expr t)
         arg_bounds out_bounds
-        (InterpE : type.interp s -> type.interp d)
+        (InterpE : type.interp t)
         (InterpE_correct
          : forall arg
                   (Harg : ZRange.type.option.is_bounded_by arg_bounds arg = true),
-            Interp e arg = InterpE arg)
+            app_curried (Interp e) arg = app_curried InterpE arg)
         rv
         (Hrv : BoundsPipeline (*with_dead_code_elimination*) with_subst01 relax_zrange e arg_bounds out_bounds = Success rv)
     : BoundsPipeline_correct_transT arg_bounds out_bounds InterpE rv.
@@ -6950,17 +6643,17 @@ Module Pipeline.
              (with_dead_code_elimination : bool := true)
              (with_subst01 : bool)
              relax_zrange
-             {s d}
-             (E : for_reification.Expr (s -> d))
+             {t}
+             (E : for_reification.Expr t)
              arg_bounds
              out_bounds
-  : ErrorT (Expr (s -> d))
+  : ErrorT (Expr (type.uncurry t))
     := let E := PrePipeline E in
        @BoundsPipeline
          (*with_dead_code_elimination*)
          with_subst01
          relax_zrange
-         s d E arg_bounds out_bounds.
+         t E arg_bounds out_bounds.
 
   Lemma BoundsPipeline_full_correct
              (with_dead_code_elimination : bool := true)
@@ -6968,8 +6661,8 @@ Module Pipeline.
              relax_zrange
              (Hrelax : forall r r' z : zrange,
                  (z <=? r)%zrange = true -> relax_zrange r = Some r' -> (z <=? r')%zrange = true)
-             {s d}
-             (E : for_reification.Expr (s -> d))
+             {t}
+             (E : for_reification.Expr t)
              arg_bounds
              out_bounds
              rv
@@ -6977,109 +6670,10 @@ Module Pipeline.
     : forall arg
              (Harg : ZRange.type.option.is_bounded_by arg_bounds arg = true),
       ZRange.type.option.is_bounded_by out_bounds (Interp rv arg) = true
-      /\ Interp rv arg = for_reification.Interp E arg.
+      /\ Interp rv arg = app_curried (for_reification.Interp E) arg.
   Proof.
     cbv [BoundsPipeline_full] in *.
     eapply BoundsPipeline_correct_trans; [ eassumption | | eassumption.. ].
-    intros; erewrite PrePipeline_correct; reflexivity.
-  Qed.
-
-  Lemma BoundsPipelineConst_correct
-             (with_dead_code_elimination : bool := true)
-             (with_subst01 : bool)
-             relax_zrange
-             (Hrelax : forall r r' z : zrange,
-                 (z <=? r)%zrange = true -> relax_zrange r = Some r' -> (z <=? r')%zrange = true)
-             {d}
-             (e : Expr d)
-             bounds
-             rv
-             (Hrv : BoundsPipelineConst (*with_dead_code_elimination*) with_subst01 relax_zrange e bounds = Success rv)
-    : ZRange.type.option.is_bounded_by bounds (Interp rv) = true
-      /\ Interp rv = Interp e.
-  Proof.
-    cbv [BoundsPipelineConst BoundsPipeline_0_or_1 Let_In] in *;
-      repeat match goal with
-             | [ H : match ?x with _ => _ end = Success _ |- _ ]
-               => destruct x eqn:?; cbv beta iota in H; [ | congruence ];
-                    let H' := fresh in
-                    inversion H as [H']; clear H; rename H' into H
-             end.
-    { intros;
-        match goal with
-        | [ H : _ = _ |- _ ]
-          => eapply CheckedPartialEvaluateWithBounds0_Correct in H;
-               [ destruct H as [H0 H1] | .. ]
-        end;
-        [
-        | eassumption || (try reflexivity).. ].
-      refine (let H' := admit (* interp correctness *) in
-              conj _ (eq_trans H' _));
-        clearbody H'.
-      { rewrite H'; eassumption. }
-      { rewrite H0.
-        exact admit. (* interp correctness *) } }
-  Qed.
-
-  Definition BoundsPipelineConst_correct_transT
-             {t}
-             out_bounds
-             (InterpE : type.interp t)
-             (rv : Expr t)
-    := ZRange.type.option.is_bounded_by out_bounds (Interp rv) = true
-       /\ Interp rv = InterpE.
-
-  Lemma BoundsPipelineConst_correct_trans
-        (with_dead_code_elimination : bool := true)
-        (with_subst01 : bool)
-        relax_zrange
-        (Hrelax
-         : forall r r' z : zrange,
-            (z <=? r)%zrange = true -> relax_zrange r = Some r' -> (z <=? r')%zrange = true)
-        {t}
-        (e : Expr t)
-        out_bounds
-        (InterpE : type.interp t)
-        (InterpE_correct : Interp e = InterpE)
-        rv
-        (Hrv : BoundsPipelineConst (*with_dead_code_elimination*) with_subst01 relax_zrange e out_bounds = Success rv)
-    : BoundsPipelineConst_correct_transT out_bounds InterpE rv.
-  Proof.
-    rewrite <- InterpE_correct.
-    eapply @BoundsPipelineConst_correct; eassumption.
-  Qed.
-
-  Definition BoundsPipelineConst_full
-             (with_dead_code_elimination : bool := true)
-             (with_subst01 : bool)
-             relax_zrange
-             {t}
-             (E : for_reification.Expr t)
-             out_bounds
-  : ErrorT (Expr t)
-    := let E := PrePipeline E in
-       @BoundsPipelineConst
-         (*with_dead_code_elimination*)
-         with_subst01
-         relax_zrange
-         t E out_bounds.
-
-  Lemma BoundsPipelineConst_full_correct
-             (with_dead_code_elimination : bool := true)
-             (with_subst01 : bool)
-             relax_zrange
-             (Hrelax : forall r r' z : zrange,
-                 (z <=? r)%zrange = true -> relax_zrange r = Some r' -> (z <=? r')%zrange = true)
-             {t}
-             (E : for_reification.Expr t)
-             out_bounds
-             rv
-             (Hrv : BoundsPipelineConst_full (*with_dead_code_elimination*) with_subst01 relax_zrange E out_bounds = Success rv)
-    : ZRange.type.option.is_bounded_by out_bounds (Interp rv) = true
-      /\ Interp rv = for_reification.Interp E.
-  Proof.
-    cbv [BoundsPipelineConst_full] in *.
-    eapply BoundsPipelineConst_correct_trans; [ eassumption | | eassumption.. ].
     intros; erewrite PrePipeline_correct; reflexivity.
   Qed.
 End Pipeline.
@@ -7176,34 +6770,15 @@ Section rcarry_mul.
           relax_zrange
           rop%Expr in_bounds out_bounds).
 
-  Notation BoundsPipelineConst rop out_bounds
-    := (Pipeline.BoundsPipelineConst
-          (*false*) true
-          relax_zrange
-          rop%Expr out_bounds).
-
   Notation BoundsPipeline_correct in_bounds out_bounds op
-    := (fun rv (rop : Expr (type.reify_type_of op%function)) Hrop
+    := (fun rv (rop : Expr (type.reify_type_of op)) Hrop
         => @Pipeline.BoundsPipeline_correct_trans
              (*false*) true
              relax_zrange
              (relax_zrange_gen_good _)
-             _ _
+             _
              rop
              in_bounds
-             out_bounds
-             op
-             Hrop rv)
-         (only parsing).
-
-  Notation BoundsPipelineConst_correct out_bounds op
-    := (fun rv (rop : Expr (type.reify_type_of op)) Hrop
-        => @Pipeline.BoundsPipelineConst_correct_trans
-             (*false*) true
-             relax_zrange
-             (relax_zrange_gen_good _)
-             _
-             rop%Expr
              out_bounds
              op
              Hrop rv)
@@ -7260,12 +6835,14 @@ Section rcarry_mul.
          (encodemod (Qnum limbwidth) (Z.pos (Qden limbwidth)) s c n (List.length c)).
 
   Definition rzero_correct
-    := BoundsPipelineConst_correct
+    := BoundsPipeline_correct
+         tt
          (Some tight_bounds)
          (zeromod (Qnum limbwidth) (Z.pos (Qden limbwidth)) s c n (List.length c)).
 
   Definition rone_correct
-    := BoundsPipelineConst_correct
+    := BoundsPipeline_correct
+         tt
          (Some tight_bounds)
          (onemod (Qnum limbwidth) (Z.pos (Qden limbwidth)) s c n (List.length c)).
 
@@ -7363,8 +6940,8 @@ Section rcarry_mul.
            (Interp raddv)
            (Interp rsubv)
            (Interp roppv)
-           (Interp rzerov)
-           (Interp ronev)
+           (Interp rzerov tt)
+           (Interp ronev tt)
            (Interp rencodev).
 
     Theorem Good : GoodT.
@@ -7382,9 +6959,12 @@ Section rcarry_mul.
                      | apply conj
                      | progress intros
                      | progress cbv [onemod zeromod]
+                     | eapply Hrzerov (* to handle diff with whether or not correctness asks for boundedness of tt *)
+                     | eapply Hronev (* to handle diff with whether or not correctness asks for boundedness of tt *)
                      | match goal with
                        | [ |- ?x = ?x ] => reflexivity
                        | [ |- ?x = ?ev ] => is_evar ev; reflexivity
+                       | [ |- ZRange.type.option.is_bounded_by tt tt = true ] => reflexivity
                        end ].
     Qed.
   End make_ring.
@@ -7400,6 +6980,9 @@ Proof. cbv [pointwise_relation]; intros; subst; trivial. Qed.
 
 Ltac peel_interp_app _ :=
   lazymatch goal with
+  | [ |- ?R' (?InterpE ?arg) (?f ?arg) ]
+    => apply fg_equal_rel; [ | reflexivity ];
+       try peel_interp_app ()
   | [ |- ?R' (Interp ?ev) (?f ?x) ]
     => let sv := type of x in
        let fx := constr:(f x) in
@@ -7420,10 +7003,9 @@ Ltac peel_interp_app _ :=
                end ] ]
   end.
 Ltac pre_cache_reify _ :=
+  cbv [app_curried];
   let arg := fresh "arg" in
-  (tryif intros arg _
-    then apply fg_equal_rel; [ | reflexivity ]
-    else hnf);
+  intros arg _;
   peel_interp_app ();
   [ lazymatch goal with
     | [ |- ?R (Interp ?ev) _ ]
@@ -7733,7 +7315,6 @@ Module X25519_64.
             base_51_encode_correct.
 
   Print Assumptions base_51_good.
-
   Import PrintingNotations.
   Print base_51_carry_mul.
 (*base_51_carry_mul =
@@ -8304,12 +7885,12 @@ Module MontgomeryReduction.
               else res.
 
     Notation BoundsPipeline_correct in_bounds out_bounds op
-      := (fun rv (rop : Expr (type.reify_type_of op%function)) Hrop
+      := (fun rv (rop : Expr (type.reify_type_of op)) Hrop
           => @Pipeline.BoundsPipeline_correct_trans
                false (* subst01 *)
                relax_zrange
                (relax_zrange_gen_good _)
-               _ _
+               _
                rop
                in_bounds
                out_bounds
